(doesn't build) Move more stuff around & start working towards actual Go semantics

src/Go.v
@@ -1,10 +1,10 @@
 Require Import PeanoNat String List FMapAVL.
 Require Import Relation_Operators Operators_Properties.
 Require Import Morphisms.
-Require Import VerdiTactics.
 Require Import StringMap.
-Require Import Mem AsyncDisk.
+Require Import VerdiTactics.
 Require Import Word.
+Require Import Mem AsyncDisk PredCrash Prog.
 
 Import ListNotations.
 
@@ -42,13 +42,23 @@ Ltac eforward H :=
     evar (v : A); specialize (H v); subst v
   end.
 
+Fixpoint all_some A (l : list (option A)) : option (list A) :=
+  match l with
+    | [] => Some []
+    | x :: xs =>
+      match x, all_some xs with
+        | Some x0, Some xs0 => Some (x0 :: xs0)
+        | _, _ => None
+      end
+  end.
+
 
 (*
 Semantics for Go
 ================
 
 * No pointer aliasing. Use pointers for types which can be mutated. (Or for everything?)
-* Ony declare variables at beginning of block
+* Disallow shadowing (good idea?)
 *)
 
 Notation W := nat. (* Assume bignums? *)
@@ -115,12 +125,12 @@ Module Go.
 
   Inductive stmt :=
   | Skip : stmt
-  | Block : scope -> stmt -> stmt
   | Seq : stmt -> stmt -> stmt
   | If : expr -> stmt -> stmt -> stmt
   | While : expr -> stmt -> stmt
   | Call : list var -> label -> list var -> stmt
   | Assign : var -> expr -> stmt
+  | Declare : var -> type -> stmt
   | DiskRead : var -> expr -> stmt
   | DiskWrite : expr -> expr -> stmt
   (* Only appears at runtime *)
@@ -129,10 +139,6 @@ Module Go.
   (* Program does not contain an InCall. Could probably be expressed directly if we had generics. *)
   Inductive source_stmt : stmt -> Prop :=
   | SSkip : source_stmt Skip
-  | SBlock :
-      forall sc a,
-        source_stmt a ->
-        source_stmt (Block sc a)
   | SSeq :
       forall a b,
         source_stmt a ->
@@ -149,12 +155,12 @@ Module Go.
         source_stmt (While cond body)
   | SCall : forall x f args, source_stmt (Call x f args)
   | SAssign : forall x e, source_stmt (Assign x e)
+  | SDeclare : forall x e, source_stmt (Declare x e)
   | SDiskRead : forall x a, source_stmt (DiskRead x a)
   | SDiskWrite : forall a v, source_stmt (DiskWrite a v).
 
   Fixpoint is_source_stmt (p : stmt) : bool :=
     match p with
-      | Block _ a => is_source_stmt a 
       | Seq a b => is_source_stmt a && is_source_stmt b
       | If cond t f => is_source_stmt t && is_source_stmt f
       | While cond body => is_source_stmt body
@@ -240,6 +246,13 @@ Module Go.
       | _, _, _ => st
     end.
 
+  Fixpoint add_many keys (output : list value) st :=
+    match keys, output with
+      | k :: keys', v :: output' =>
+        let st' := StringMap.add k v st in
+        add_many keys' output' st'
+      | _, _ => st
+    end.
 
   Fixpoint mapM A B (f : A -> option B) ls :=
     match ls with
@@ -321,9 +334,9 @@ Module Go.
 
   Record OperationalSpec := {
     ArgVars : list var;
-    RetVar : option var;
+    RetVars : list var;
     Body : stmt;
-    ret_not_in_args : is_none_or_not_in RetVar ArgVars = true;
+    (* ret_not_in_args : dont_intersect RetVars ArgVars = true; *)
     args_no_dup : is_no_dup ArgVars = true;
     body_source : is_source_stmt Body = true;
     (* TODO syntax_ok with is_actual_args_no_dup *)
@@ -339,5 +352,474 @@ Module Go.
     RetV : var;
   }.
 
+  Section EnvSection.
+
+    Variable env : Env.
+
+    Definition sel T m := fun k => StringMap.find k m : option T.
+
+    Fixpoint make_map {elt} keys values :=
+      match keys, values with
+        | k :: keys', v :: values' => StringMap.add k v (make_map keys' values')
+        | _, _ => @StringMap.empty elt
+      end.
+
+    Eval hnf in rawdisk.
+
+    Definition maybe_add V k (v : V) m :=
+      match k with
+        | None => m
+        | Some kk => StringMap.add kk v m
+      end.
+
+
+    Inductive RunsTo : stmt -> state -> state -> Prop :=
+    | RunsToSkip : forall st,
+                     RunsTo Skip st st
+    | RunsToSeq : forall a b st st' st'',
+                    RunsTo a st st' ->
+                    RunsTo b st' st'' ->
+                    RunsTo (Seq a b) st st'
+    | RunsToIfTrue : forall cond t f st st',
+                       is_true (snd st) cond ->
+                       RunsTo t st st' ->
+                       RunsTo (If cond t f) st st'
+    | RunsToIfFalse : forall cond t f st st',
+                        is_false (snd st) cond ->
+                        RunsTo f st st' ->
+                        RunsTo (If cond t f) st st'
+    | RunsToWhileTrue : forall cond body st st' st'',
+                          let loop := While cond body in
+                          is_true (snd st) cond ->
+                          RunsTo body st st' ->
+                          RunsTo loop st' st'' ->
+                          RunsTo loop st st''
+    | RunsToWhileFalse : forall cond body st,
+                           let loop := While cond body in
+                           is_false (snd st) cond ->
+                           RunsTo loop st st
+    | RunsToAssign : forall x e d s s' v,
+                       (* rhs can't be a mutable object, to prevent aliasing *)
+                       eval s e = Some v ->
+                       can_alias (type_of v) = true ->
+                       s' = StringMap.add x v s ->
+                       RunsTo (Assign x e) (d, s) (d, s')
+    | RunsToDiskRead : forall x ae a d s s' v vs,
+                         eval s ae = Some (Val Num a) ->
+                         d a = Some (v, vs) ->
+                         s' = StringMap.add x (Val DiskBlock v) s ->
+                         RunsTo (DiskRead x ae) (d, s) (d, s')
+    | RunsToDiskWrite : forall ae a ve v (d : rawdisk) d' s v0 v0s,
+                          eval s ae = Some (Val Num a) ->
+                          eval s ve = Some (Val DiskBlock v) ->
+                          d a = Some (v0, v0s) ->
+                          d' = upd d a (v, v0 :: v0s) ->
+                          RunsTo (DiskWrite ae ve) (d, s) (d', s)
+    | RunsToCallOp : forall retvars f args s spec d d' input callee_s' ret,
+                       StringMap.find f env = Some spec ->
+                       source_stmt (Body spec) ->
+                       length args = length (ArgVars spec) ->
+                       mapM (sel s) args = Some input ->
+                       let callee_s := make_map (ArgVars spec) input in
+                       RunsTo (Body spec) (d, callee_s) (d', callee_s') ->
+                       all_some (List.map (fun rv => sel callee_s' rv) (RetVars spec)) = Some ret ->
+                       let output := List.map (sel callee_s') (ArgVars spec) in
+                       let s' := add_remove_many args input output s in
+                       let s' := add_many retvars ret s' in
+                       RunsTo (Call retvars f args) (d, s) (d', s').
+
+    Inductive Step : state * stmt -> state * stmt -> Prop :=
+    | StepSeq1 : forall a a' b st st',
+                   Step (st, a) (st', a') ->
+                   Step (st, Seq a b) (st', Seq a' b)
+    | StepSeq2 : forall a st,
+                   Step (st, Seq Skip a) (st, a)
+    | StepIfTrue : forall cond t f st,
+                     is_true (snd st) cond ->
+                     Step (st, If cond t f) (st, t)
+    | StepIfFalse : forall cond t f st,
+                      is_false (snd st) cond ->
+                      Step (st, If cond t f) (st, f)
+    | StepWhileTrue : forall cond body st,
+                        let loop := While cond body in
+                        is_true (snd st) cond ->
+                        Step (st, loop) (st, Seq body loop)
+    | StepWhileFalse : forall cond body st,
+                         let loop := While cond body in
+                         is_false (snd st) cond ->
+                         Step (st, loop) (st, Skip)
+    | StepAssign : forall x e d s s' v,
+                     (* rhs can't be a mutable object, to prevent aliasing *)
+                     eval s e = Some v ->
+                     can_alias v = true ->
+                     s' = add x v s ->
+                     Step (d, s, Assign x e) (d, s', Skip)
+    | StepDiskRead : forall x ae a d s s' v vs,
+                       eval s ae = Some (Num a) ->
+                       d a = Some (v, vs) ->
+                       s' = add x (Block v) s ->
+                       Step (d, s, DiskRead x ae) (d, s', Skip)
+    | StepDiskWrite : forall ae a ve v d d' s v0 v0s,
+                        eval s ae = Some (Num a) ->
+                        eval s ve = Some (Block v) ->
+                        d a = Some (v0, v0s) ->
+                        d' = upd d a (v, v0 :: v0s) ->
+                        Step (d, s, DiskWrite ae ve) (d', s, Skip)
+    | StepStartCall :
+        forall x f args s spec d input,
+          StringMap.find f env = Some spec ->
+          SourceStmt (Body spec) ->
+          length args = length (ArgVars spec) ->
+          mapM (sel s) args = Some input ->
+          let callee_s := make_map (ArgVars spec) input in
+          Step (d, s, Call x f args) (d, callee_s, InCall s spec.(ArgVars) spec.(RetVar) args x spec.(Body))
+    | StepInCall :
+        forall st p st' p' s0 argvars retvar args ret,
+          Step (st, p) (st', p') ->
+          Step (st, InCall s0 argvars retvar args ret p) (st', InCall s0 argvars retvar args ret p')
+    | StepEndCall :
+        forall callee_s' s d input retval argvars retvar args ret,
+          mapM (sel s) args = Some input ->
+          length args = length argvars ->
+          match retvar with
+            | None => ret = None
+            | Some rv => sel callee_s' rv = Some retval
+          end ->
+          let output := List.map (sel callee_s') argvars in
+          let s' := add_remove_many args input output s in
+          let s' := maybe_add ret retval s' in
+          Step (d, callee_s', InCall s argvars retvar args ret Skip) (d, s', Skip).
+
+    Inductive Outcome :=
+    | EFailed
+    | EFinished (st : rawdisk * Locals)
+    | ECrashed (d : rawdisk).
+
+    Inductive CrashStep : Stmt -> Prop :=
+    | CrashSeq1 : forall a b,
+                    CrashStep a ->
+                    CrashStep (Seq a b)
+    | CrashInCall : forall s argvars retvar args ret p,
+                      CrashStep p ->
+                      CrashStep (InCall s argvars retvar args ret p)
+    | CrashRead : forall x a,
+                    CrashStep (DiskRead x a)
+    | CrashWrite : forall a v,
+                     CrashStep (DiskWrite a v).
+
+    Definition is_final (sst : State * Stmt) : Prop :=
+      snd sst = Skip.
+
+    Hint Unfold is_final.
+
+    Inductive Exec : State * Stmt -> Outcome -> Prop :=
+    | EXStep : forall sst sst' out,
+                 Step sst sst' ->
+                 Exec sst' out ->
+                 Exec sst out
+    | EXFail : forall sst,
+                 (~exists st' p', Step sst (st', p')) ->
+                 ~is_final sst ->
+                 Exec sst EFailed
+    | EXCrash : forall d s p,
+                  CrashStep p ->
+                  Exec (d, s, p) (ECrashed d)
+    | EXDone : forall st,
+                 Exec (st, Skip) (EFinished st).
+
+    Hint Constructors Exec RunsTo Step.
+
+    Hint Constructors clos_refl_trans_1n.
+
+    Definition rt1n_front := Relation_Operators.rt1n_trans.
+
+    Lemma rt1n_trans' : forall A R x y z,
+                          clos_refl_trans_1n A R x y ->
+                          clos_refl_trans_1n A R y z ->
+                          clos_refl_trans_1n A R x z.
+    Proof.
+      eauto using clos_rt_rt1n, clos_rt1n_rt, rt_trans.
+    Qed.
+
+    Hint Extern 1 (clos_refl_trans_1n _ _ ?x ?y) =>
+    match goal with
+      | _ => is_evar x; fail 1
+      | _ => is_evar y; fail 1
+      | _ => eapply rt1n_trans'
+    end.
+
+
+    Ltac do_inv :=
+      match goal with
+        | [ H : Step _ _ |- _ ] => invc H; eauto
+        | [ H : clos_refl_trans_1n _ _ _ _ |- _ ] => invc H; eauto
+      end.
+
+    Lemma steps_incall :
+      forall s0 argvars retvar args ret st p st' p',
+        Step^* (st, p) (st', p') ->
+        Step^* (st, InCall s0 argvars retvar args ret p) (st', InCall s0 argvars retvar args ret p').
+    Proof.
+      intros.
+      prep_induction H; induction H; intros; subst.
+      - find_inversion. eauto.
+      - destruct y. eauto.
+    Qed.
+    Hint Resolve steps_incall.
+
+    Lemma steps_sequence :
+      forall p0 st p st' p',
+        Step^* (st, p) (st', p') ->
+        Step^* (st, Seq p p0) (st', Seq p' p0).
+    Proof.
+      intros.
+      prep_induction H; induction H; intros; subst.
+      - find_inversion. eauto.
+      - destruct y. eauto.
+    Qed.
+    Hint Resolve steps_sequence.
+
+    (* For some reason (probably involving tuples), the [Hint Constructors] isn't enough. *)
+    Hint Extern 1 (Step (_, Assign _ _) _) =>
+    eapply StepAssign.
+    Hint Extern 1 (Step (_, DiskRead _ _) _) =>
+    eapply StepDiskRead.
+    Hint Extern 1 (Step (_, DiskWrite _ _) _) =>
+    eapply StepDiskWrite.
+    Hint Extern 1 (Step (_, Call _ _ _) _) =>
+    eapply StepStartCall.
+    Hint Extern 1 (Step (_, InCall _ _ _ _ _ _) _) =>
+    eapply StepEndCall.
+
+    Theorem RunsTo_Steps :
+      forall p st st',
+        RunsTo p st st' ->
+        Step^* (st, p) (st', Skip).
+    Proof.
+      intros.
+      induction H; subst_definitions; subst; eauto 10.
+    Qed.
+
+    Inductive RunsTo_InCall : Stmt -> State -> State -> Prop :=
+    (* We'd have to duplicate all the [RunsTo] constructors which are recursive anyway *)
+    | RunsToICSkip : forall st,
+                       RunsTo_InCall Skip st st
+    | RunsToICSeq : forall a b st st' st'',
+                      RunsTo_InCall a st st' ->
+                      RunsTo_InCall b st' st'' ->
+                      RunsTo_InCall (Seq a b) st st''
+    | RunsToICIfTrue : forall cond t f st st',
+                         is_true (snd st) cond ->
+                         RunsTo_InCall t st st' ->
+                         RunsTo_InCall (If cond t f) st st'
+    | RunsToICIfFalse : forall cond t f st st',
+                          is_false (snd st) cond ->
+                          RunsTo_InCall f st st' ->
+                          RunsTo_InCall (If cond t f) st st'
+    | RunsToICWhileTrue : forall cond body st st' st'',
+                            let loop := While cond body in
+                            is_true (snd st) cond ->
+                            RunsTo_InCall body st st' ->
+                            RunsTo_InCall loop st' st'' ->
+                            RunsTo_InCall loop st st''
+    | RunsToICWhileFalse : forall cond body st,
+                             let loop := While cond body in
+                             is_false (snd st) cond ->
+                             RunsTo_InCall loop st st
+    | RunsToICAssign : forall x e d s s' v,
+                         (* rhs can't be a mutable object, to prevent aliasing *)
+                         eval s e = Some v ->
+                         can_alias v = true ->
+                         s' = add x v s ->
+                         RunsTo_InCall (Assign x e) (d, s) (d, s')
+    | RunsToICDiskRead : forall x ae a d s s' v vs,
+                           eval s ae = Some (Num a) ->
+                           d a = Some (v, vs) ->
+                           s' = add x (Block v) s ->
+                           RunsTo_InCall (DiskRead x ae) (d, s) (d, s')
+    | RunsToICDiskWrite : forall ae a ve v d d' s v0 v0s,
+                            eval s ae = Some (Num a) ->
+                            eval s ve = Some (Block v) ->
+                            d a = Some (v0, v0s) ->
+                            d' = upd d a (v, v0 :: v0s) ->
+                            RunsTo_InCall (DiskWrite ae ve) (d, s) (d', s)
+    | RunsToICCallOp : forall x f args s spec d d' input callee_s' ret,
+                         StringMap.find f env = Some spec ->
+                         SourceStmt (Body spec) ->
+                         length args = length (ArgVars spec) ->
+                         mapM (sel s) args = Some input ->
+                         let callee_s := make_map (ArgVars spec) input in
+                         RunsTo_InCall (Body spec) (d, callee_s) (d', callee_s') ->
+                         match RetVar spec with
+                           | None => x = None
+                           | Some rv => sel callee_s' rv = Some ret
+                         end ->
+                         let output := List.map (sel callee_s') (ArgVars spec) in
+                         let s' := add_remove_many args input output s in
+                         let s' := maybe_add x ret s' in
+                         RunsTo_InCall (Call x f args) (d, s) (d', s')
+    | RunsToInCall : forall s0 x args (argvars : list var) retvar input ret p d d' callee_s callee_s',
+                       mapM (sel s0) args = Some input ->
+                       length args = length argvars ->
+                       match retvar with
+                         | None => x = None
+                         | Some rv => sel callee_s' rv = Some ret
+                       end ->
+                       let output := List.map (sel callee_s') argvars in
+                       let s' := add_remove_many args input output s0 in
+                       let s' := maybe_add x ret s' in
+                       RunsTo_InCall p (d, callee_s) (d', callee_s') ->
+                       RunsTo_InCall (InCall s0 argvars retvar args x p) (d, callee_s) (d', s').
+
+    Hint Constructors SourceStmt.
+
+    Lemma SourceStmt_RunsToInCall_RunsTo :
+      forall p,
+        SourceStmt p ->
+        forall st st',
+          RunsTo_InCall p st st' ->
+          RunsTo p st st'.
+    Proof.
+      induction 2; intros; subst_definitions; invc H; eauto.
+    Qed.
+
+    Hint Resolve SourceStmt_RunsToInCall_RunsTo.
+
+    Hint Constructors RunsTo_InCall.
+
+    Lemma RunsTo_RunsToInCall :
+      forall p st st',
+        RunsTo p st st' ->
+        RunsTo_InCall p st st'.
+    Proof.
+      induction 1; intros; subst_definitions; eauto.
+    Qed.
+
+    Hint Resolve RunsTo_RunsToInCall.
+
+    Ltac inv_runsto :=
+      match goal with
+        | [ H: RunsTo ?c _ _ |- _ ] =>
+          (is_var c; fail 1) ||
+                             invc H
+        | [ H: RunsTo_InCall _ _ _ |- _ ] =>
+          invc H
+      end.
+
+    Lemma Step_RunsTo :
+      forall st p st' p' st'',
+        Step (st, p) (st', p') ->
+        RunsTo_InCall p' st' st'' ->
+        RunsTo_InCall p st st''.
+    Proof.
+      intros.
+      prep_induction H0; induction H0; intros; subst_definitions; subst; do_inv.
+      - subst_definitions. eauto.
+      - eapply RunsToICCallOp; eauto. assert (Some input = Some input0) by congruence. find_inversion. auto.
+      - destruct st. eapply RunsToInCall; eauto.
+    Qed.
+
+    Hint Resolve Step_RunsTo.
+
+    Theorem Steps_RunsTo' :
+      forall p st st',
+        Step^* (st, p) (st', Skip) ->
+        RunsTo_InCall p st st'.
+    Proof.
+      intros.
+      prep_induction H; induction H; intros; subst.
+      - find_inversion. eauto.
+      - destruct y. eauto.
+    Qed.
+
+    Theorem Steps_RunsTo :
+      forall p st st',
+        SourceStmt p ->
+        Step^* (st, p) (st', Skip) ->
+        RunsTo p st st'.
+    Proof.
+      intros.
+      eauto using Steps_RunsTo'.
+    Qed.
+
+    Theorem ExecFinished_Steps : forall p st st',
+                                   Exec (st, p) (EFinished st') ->
+                                   Step^* (st, p) (st', Skip).
+    Proof.
+      intros.
+      prep_induction H; induction H; intros; subst; try discriminate.
+      + destruct sst'. eauto.
+      + repeat find_inversion. eauto.
+    Qed.
+
+    Theorem Steps_ExecFinished : forall p st st',
+                                   Step^* (st, p) (st', Skip) ->
+                                   Exec (st, p) (EFinished st').
+    Proof.
+      intros.
+      prep_induction H; induction H; intros; subst; try discriminate.
+      + find_inversion. eauto.
+      + destruct y. eauto.
+    Qed.
+
+    Theorem ExecCrashed_Steps : forall p st d',
+                                  Exec (st, p) (ECrashed d') ->
+                                  exists s' p', Step^* (st, p) (d', s', p') /\ CrashStep p'.
+    Proof.
+      intros.
+      prep_induction H; induction H; intros; subst; try discriminate.
+      + destruct sst'. specialize (IHExec _ _ _ eq_refl eq_refl). repeat deex. eauto 8.
+      + find_inversion. find_inversion. eauto 8.
+    Qed.
+
+    Theorem Steps_ExecCrashed : forall st p d' s' p',
+                                  Step^* (st, p) (d', s', p') ->
+                                  CrashStep p' ->
+                                  Exec (st, p) (ECrashed d').
+    Proof.
+      intros.
+      destruct st.
+      prep_induction H; induction H; intros; subst.
+      + repeat find_inversion. eauto.
+      + destruct y. destruct s. eauto.
+    Qed.
+
+    Theorem ExecFailed_Steps :
+      forall st p,
+        Exec (st, p) EFailed ->
+        exists st' p', Step^* (st, p) (st', p') /\ ~is_final (st', p') /\ ~exists st'' p'', Step (st', p') (st'', p'').
+    Proof.
+      intros.
+      unfold is_final; simpl.
+      prep_induction H; induction H; intros; subst; try discriminate; eauto.
+      - destruct sst'. repeat eforward IHExec. repeat conclude IHExec eauto. repeat deex.
+        eauto 10.
+    Qed.
+
+    Theorem Steps_ExecFailed :
+      forall st p st' p',
+        ~is_final (st', p') ->
+        (~exists st'' p'', Step (st', p') (st'', p'')) ->
+        Step^* (st, p) (st', p') ->
+        Exec (st, p) EFailed.
+    Proof.
+      induction 3; eauto.
+    Qed.
+
+    Lemma Steps_Seq :
+      forall p1 p2 p' st st'',
+        Step^* (st, Seq p1 p2) (st'', p') ->
+        (exists p1', Step^* (st, p1) (st'', p1') /\ p' = Seq p1' p2) \/
+        (exists st', Step^* (st, p1) (st', Skip) /\ Step^* (st', p2) (st'', p')).
+    Proof.
+      intros.
+      prep_induction H; induction H; intros; subst.
+      - find_inversion. eauto.
+      - destruct y. invc H.
+        + destruct (IHclos_refl_trans_1n _ _ _ _ _ eq_refl eq_refl); eauto; deex; eauto.
+        + eauto.
+    Qed.
+
+  End EnvSection.
   
 End Go.
